progress on ed25519

code/curve25519/Hacl.EC.Format.fst
@@ -112,13 +112,14 @@ private let upd_5' output output0 output1 output2 output3 output4 =
 
 #reset-options "--initial_fuel 0 --max_fuel 0 --z3rlimit 400"
 
-private val fexpand: output:felem -> input:uint8_p{length input = 32} -> Stack unit
+val fexpand: output:felem -> input:uint8_p{length input = 32} -> Stack unit
   (requires (fun h -> Buffer.live h output /\ Buffer.live h input))
   (ensures (fun h0 _ h1 -> Buffer.live h0 output /\ Buffer.live h0 input
     /\ Buffer.live h1 output /\ modifies_1 output h0 h1
     /\ Hacl.Spec.EC.AddAndDouble.red_513 (as_seq h1 output)
+    /\ Hacl.Spec.EC.AddAndDouble.(bounds (as_seq h1 output) p51 p51 p51 p51 p51)
     /\ as_seq h1 output == Hacl.Spec.EC.Format.fexpand_spec (as_seq h0 input)))
-private let fexpand output input =
+let fexpand output input =
   let h = ST.get() in
   Seq.lemma_eq_intro (Seq.slice (as_seq h input) 0 8) (as_seq h (Buffer.sub input 0ul 8ul));
   Seq.lemma_eq_intro (Seq.slice (as_seq h input) 6 14) (as_seq h (Buffer.sub input 6ul 8ul));
