code/experimental/ed25519/Hacl.Impl.Ed25519.PointCompress.fst
@@ -5,7 +5,7 @@ open Hacl.UInt64
 open Hacl.Bignum25519
 
 
-#reset-options "--max_fuel 0 --z3rlimit 20"
+#reset-options "--max_fuel 0 --z3rlimit 100"
 
 let hint8_p = buffer Hacl.UInt8.t
 let hint64_p = buffer Hacl.UInt64.t
@@ -14,10 +14,10 @@ let op_String_Access h b = Hacl.Spec.Endianness.reveal_sbytes (as_seq h b)
 open FStar.Mul
 
 private let lemma_distr_4 a b c d e : Lemma (a * (b + c + d + e) == a * b + a * c + a * d + a * e)
-  = ()
+  = Math.Lemmas.distributivity_add_right a (b + c + d) e;
+    Math.Lemmas.distributivity_add_right a (b + c) d;
+    Math.Lemmas.distributivity_add_right a (b) c
 
-
-#reset-options "--max_fuel 0 --z3rlimit 20"
 
 private let lemma_x_mod_2 (a:nat) (b:nat) (c:nat) (d:nat) (e:nat) : 
   Lemma ((a + pow2 51 * b + pow2 102 * c + pow2 153 * d + pow2 204 * e) % 2 = a % 2)
@@ -32,6 +32,7 @@ private let lemma_x_mod_2 (a:nat) (b:nat) (c:nat) (d:nat) (e:nat) :
     Math.Lemmas.paren_mul_right 2 (pow2 203) e;
     Math.Lemmas.modulo_addition_lemma a 2 ((pow2 50 * b)+(pow2 101 * c)+(pow2 152 * d)+(pow2 203 * e))
 
+
 private val x_mod_2:
   x:felem ->
   Stack Hacl.UInt64.t
@@ -41,11 +42,16 @@ private val x_mod_2:
                                + pow2 51 * v (Seq.index s 1)
                                + pow2 102 * v (Seq.index s 2)
                                + pow2 153 * v (Seq.index s 3)
-                               + pow2 204 * v (Seq.index s 4) == seval (as_seq h x))))))
-    (ensures (fun h0 z h1 -> h0 == h1 /\ live h0 x /\
-      v z = seval (as_seq h0 x) % 2))
+                               + pow2 204 * v (Seq.index s 4) < pow2 255 - 19)))))
+    (ensures (fun h0 z h1 -> h0 == h1 /\ live h0 x /\ v z = seval (as_seq h0 x) % 2))
 let x_mod_2 x =
   let h = ST.get() in
+  Hacl.Bignum25519.lemma_reveal_seval (as_seq h x);
+  Math.Lemmas.modulo_lemma (let s = as_seq h x in v (Seq.index s 0)
+                               + pow2 51 * v (Seq.index s 1)
+                               + pow2 102 * v (Seq.index s 2)
+                               + pow2 153 * v (Seq.index s 3)
+                               + pow2 204 * v (Seq.index s 4)) Spec.Curve25519.prime;
   lemma_x_mod_2 (v (get h x 0)) (v (get h x 1)) (v (get h x 2)) (v (get h x 3)) (v (get h x 4));
   let x0 = x.(0ul) in
   let z  = x0 &^ 1uL in
@@ -54,18 +60,94 @@ let x_mod_2 x =
   z
 
 
-val point_compress:
+
+private
+val add_sign_spec:
+  out:Seq.seq Hacl.UInt8.t{Seq.length out = 32 /\ Endianness.little_endian out < pow2 255} ->
+  x:Hacl.UInt64.t{v x < 2} ->  
+  GTot (s:Seq.seq Hacl.UInt8.t{Seq.length s = 32 /\ Endianness.little_endian s == Endianness.little_endian out + pow2 255 * v x})
+#reset-options "--max_fuel 0 --z3rlimit 100"
+let add_sign_spec out x =
+  assert_norm(pow2 7 = 128);
+  assert_norm(pow2 8 = 256);
+  assert_norm(pow2 248 = 0x100000000000000000000000000000000000000000000000000000000000000);
+  assert_norm(pow2 255 = 0x8000000000000000000000000000000000000000000000000000000000000000);
+  assert_norm(pow2 256 = 0x10000000000000000000000000000000000000000000000000000000000000000);
+  let xbyte = Hacl.Cast.sint64_to_sint8 x in
+  Math.Lemmas.modulo_lemma (v x) (pow2 8);
+  Seq.lemma_eq_intro out (Seq.append (Seq.slice out 0 31) (Seq.slice out 31 32));
+  Endianness.lemma_little_endian_is_bounded (Seq.slice (out) 0 31);
+  Endianness.little_endian_append (Seq.slice (out) 0 31) (Seq.slice (out) 31 32);
+  let o31 = Seq.index out (31) in
+  Seq.lemma_eq_intro (Seq.slice out 31 32) (Seq.create 1 o31);
+  Endianness.little_endian_singleton o31;
+  assert(Endianness.little_endian (out) == Endianness.little_endian (Seq.slice (out) 0 31)  + pow2 248 * (Hacl.UInt8.v (Seq.index (out) 31)));
+  let o31' = Hacl.UInt8.(o31 +%^ (xbyte <<^ 7ul)) in
+  Math.Lemmas.modulo_lemma (Hacl.UInt8.v xbyte * pow2 7) (pow2 8);
+  assert(Hacl.UInt8.v o31 < 128);
+  Math.Lemmas.modulo_lemma (Hacl.UInt8.v o31 + (Hacl.UInt8.v xbyte * pow2 7)) (pow2 8);
+  let out' = Seq.upd out 31 o31' in
+  Seq.lemma_eq_intro (Seq.slice (out) 0 31) (Seq.slice (out') 0 31);
+  Seq.lemma_eq_intro out' (Seq.append (Seq.slice out 0 31) (Seq.slice out' 31 32));
+  Seq.lemma_eq_intro (Seq.slice out' 31 32) (Seq.create 1 o31');
+  Endianness.little_endian_singleton o31';
+  Endianness.little_endian_append (Seq.slice (out') 0 31) (Seq.slice (out') 31 32);
+  out'
+  
+
+[@ "substitute"]
+private
+val add_sign:
   out:hint8_p{length out = 32} ->
-  p:Hacl.Impl.Ed25519.ExtPoint.point ->
+  x:Hacl.UInt64.t{v x < 2} ->
   Stack unit
-    (requires (fun h -> live h out /\ live h p))
-    (ensures (fun h0 _ h1 -> live h0 out /\ live h0 p /\ 
-      live h1 out /\ modifies_1 out h0 h1 /\
-      h1.[out] == Spec.point_compress (Hacl.Impl.Ed25519.ExtPoint.as_point h0 p)
+    (requires (fun h -> live h out /\ Endianness.little_endian (as_seq h out) < pow2 255))
+    (ensures (fun h0 _ h1 -> live h0 out /\ live h1 out /\ modifies_1 out h0 h1
+      /\ Endianness.little_endian (as_seq h1 out) == Endianness.little_endian (as_seq h0 out) + pow2 255 * v x))
+[@ "substitute"]
+let add_sign out x =
+  let h0 = ST.get() in
+  let xbyte = Hacl.Cast.sint64_to_sint8 x in
+  let o31 = out.(31ul) in
+  out.(31ul) <- Hacl.UInt8.(o31 +%^ (xbyte <<^ 7ul));
+  let h1 = ST.get() in
+  assert(as_seq h1 out == add_sign_spec (as_seq h0 out) x)
+
+
+[@ "substitute"]
+private
+val point_compress_:
+  tmp:buffer Hacl.UInt64.t{length tmp = 15} ->
+  p:Hacl.Impl.Ed25519.ExtPoint.point{disjoint tmp p} ->
+  Stack unit
+    (requires (fun h -> live h tmp /\ live h p
+      /\ red_513 (as_seq h (Hacl.Impl.Ed25519.ExtPoint.getx p))
+      /\ red_513 (as_seq h (Hacl.Impl.Ed25519.ExtPoint.gety p))
+      /\ red_513 (as_seq h (Hacl.Impl.Ed25519.ExtPoint.getz p))
+      /\ red_513 (as_seq h (Hacl.Impl.Ed25519.ExtPoint.gett p))
+      ))
+    (ensures (fun h0 _ h1 -> live h0 p /\ 
+      live h1 tmp /\ modifies_1 tmp h0 h1 /\
+      (let s = as_seq h1 (Buffer.sub tmp 5ul 5ul) in
+       let s' = as_seq h1 (Buffer.sub tmp 10ul 5ul) in
+       let x = Hacl.Bignum25519.seval (as_seq h0 (Hacl.Impl.Ed25519.ExtPoint.getx p)) in
+       let y = Hacl.Bignum25519.seval (as_seq h0 (Hacl.Impl.Ed25519.ExtPoint.gety p)) in
+       let z = Hacl.Bignum25519.seval (as_seq h0 (Hacl.Impl.Ed25519.ExtPoint.getz p)) in
+        v (Seq.index s 0) + pow2 51 * v (Seq.index s 1)
+        + pow2 102 * v (Seq.index s 2) + pow2 153 * v (Seq.index s 3)
+        + pow2 204 * v (Seq.index s 4) < Spec.Curve25519.prime /\
+        v (Seq.index s' 0) + pow2 51 * v (Seq.index s' 1)
+        + pow2 102 * v (Seq.index s' 2) + pow2 153 * v (Seq.index s' 3)
+        + pow2 204 * v (Seq.index s' 4) < Spec.Curve25519.prime /\
+        Hacl.Bignum25519.red_51 s /\
+        Hacl.Bignum25519.red_51 s' /\
+        Hacl.Bignum25519.seval s == Spec.Curve25519.(x `fmul` (z ** (prime - 2))) /\
+        Hacl.Bignum25519.seval s' == Spec.Curve25519.(y `fmul` (z ** (prime - 2))))
     ))
-let point_compress out p =
-  push_frame();
-  let tmp  = create (Hacl.Cast.uint64_to_sint64 0uL) 15ul in
+#reset-options "--max_fuel 0 --z3rlimit 100"
+[@ "substitute"]
+let point_compress_ tmp p =
+  let h0 = ST.get() in
   let zinv = Buffer.sub tmp 0ul  5ul in
   let x    = Buffer.sub tmp 5ul  5ul in
   let out  = Buffer.sub tmp 10ul 5ul in
@@ -73,11 +155,66 @@ let point_compress out p =
   let py   = Hacl.Impl.Ed25519.ExtPoint.gety p in
   let pz   = Hacl.Impl.Ed25519.ExtPoint.getz p in
   Hacl.Bignum25519.inverse  zinv pz;
+  let h = ST.get() in
+  no_upd_lemma_1 h0 h zinv x;
+  no_upd_lemma_1 h0 h zinv out;
+  no_upd_lemma_1 h0 h zinv px;
+  no_upd_lemma_1 h0 h zinv py;
+  no_upd_lemma_1 h0 h zinv pz;
+  Hacl.Bignum25519.lemma_red_513_is_red_53 (as_seq h px);
+  Hacl.Bignum25519.lemma_red_513_is_red_5413 (as_seq h zinv);
   Hacl.Bignum25519.fmul x   px zinv;
+  let hh = ST.get() in
+  Hacl.Bignum25519.lemma_reveal_seval (as_seq hh x);
+  assert(Hacl.Bignum25519.seval (as_seq hh x) < Spec.Curve25519.prime);
   Hacl.Bignum25519.reduce x;
+  let h' = ST.get() in
+  no_upd_lemma_1 h h' x zinv;
+  no_upd_lemma_1 h h' x out;
+  no_upd_lemma_1 h h' x px;
+  no_upd_lemma_1 h h' x py;
+  no_upd_lemma_1 h h' x pz;
+  Hacl.Bignum25519.lemma_red_513_is_red_53 (as_seq h' py);
   Hacl.Bignum25519.fmul out py zinv;
+  let h'' = ST.get() in
   Hacl.Bignum25519.reduce out;
-  let b = x.(0ul) &^ 1uL in
-  let out4 = out.(4ul) in
-  out.(4ul) <- out4 +^ (b <<^ 51ul);
+  let h1 = ST.get() in
+  assert(Hacl.Bignum25519.seval (as_seq h1 out) < Spec.Curve25519.prime);
+  no_upd_lemma_1 h' h1 out x;
+  no_upd_lemma_1 h' h1 out zinv;
+  no_upd_lemma_1 h' h1 out px;
+  no_upd_lemma_1 h' h1 out py;
+  no_upd_lemma_1 h' h1 out pz;
+  assert(modifies_1 tmp h0 h1)
+
+
+#reset-options "--max_fuel 0 --z3rlimit 200"
+
+val point_compress:
+  out:hint8_p{length out = 32} ->
+  p:Hacl.Impl.Ed25519.ExtPoint.point ->
+  Stack unit
+    (requires (fun h -> live h out /\ live h p
+      /\ red_513 (as_seq h (Hacl.Impl.Ed25519.ExtPoint.getx p))
+      /\ red_513 (as_seq h (Hacl.Impl.Ed25519.ExtPoint.gety p))
+      /\ red_513 (as_seq h (Hacl.Impl.Ed25519.ExtPoint.getz p))
+      /\ red_513 (as_seq h (Hacl.Impl.Ed25519.ExtPoint.gett p))
+      ))
+    (ensures (fun h0 _ h1 -> live h0 out /\ live h0 p /\ 
+      live h1 out /\ modifies_1 out h0 h1 /\
+      h1.[out] == Spec.Ed25519.point_compress (Hacl.Impl.Ed25519.ExtPoint.as_point h0 p)
+    ))
+let point_compress z p =
+  let h0 = ST.get() in
+  push_frame();
+  let tmp  = create (Hacl.Cast.uint64_to_sint64 0uL) 15ul in
+  let zinv = Buffer.sub tmp 0ul  5ul in
+  let x    = Buffer.sub tmp 5ul  5ul in
+  let out  = Buffer.sub tmp 10ul 5ul in
+  point_compress_ tmp p;
+  let b = x_mod_2 x in
+  Hacl.Impl.Store51.store_51 z out;
+  add_sign z b;
+  let h = ST.get() in
+  Endianness.lemma_little_endian_inj (as_seq h z) (Spec.Ed25519.point_compress (Hacl.Impl.Ed25519.ExtPoint.as_point h0 p));
   pop_frame()
